src/coq/Utils/MonadEq1Laws.v
@@ -1,0 +1,67 @@
+From Coq Require Import
+     Morphisms.
+
+From ITree Require Import
+     Basics.Monad.
+
+From ExtLib Require Import
+     Structures.Monads.
+
+From Vellvm.Utils Require Import MonadExcLaws.
+
+Section Laws.
+
+  Context (M : Type -> Type).
+  Context {Eq1 : @Eq1 M}.
+  Context {Monad : Monad M}.
+
+  Local Open Scope monad_scope.
+
+  Class Eq1_ret_inv : Prop :=
+    { eq1_ret_ret : forall {A} (x y : A), ret x ≈ ret y -> x = y }.
+
+End Laws.
+
+Open Scope monad_scope.
+
+Section Either.
+  Variable E : Type.
+
+  Lemma eq1_ret_ret_either:
+    forall {A} (x y : A), (ret x : sum E A) ≈ ret y -> x = y.
+  Proof.
+    intros A x y EQ.
+    unfold Monad.eq1, Eq1_either in EQ.
+    inversion EQ.
+    reflexivity.
+  Qed.
+
+  Global Instance Eq1_ret_inv_either : Eq1_ret_inv (sum E) :=
+    { eq1_ret_ret := fun a => eq1_ret_ret_either }.
+
+End Either.
+
+Section EitherT.
+  Variable E : Type.
+  Variable M : Type -> Type.
+  Context {HM : Monad M}.
+  Context {EQM : Eq1 M}.
+  Context {RINV : @Eq1_ret_inv M EQM HM}.
+
+  Import EitherMonad.
+
+  Lemma eq1_ret_ret_eitherT:
+    forall {A} (x y : A), (ret x : eitherT E M A) ≈ ret y -> x = y.
+  Proof.
+    intros A x y EQ.
+    unfold Monad.eq1, Eq1_eitherT in EQ.
+    destruct RINV.
+    specialize (eq1_ret_ret0 _ _ _ EQ).
+    inversion eq1_ret_ret0.
+    reflexivity.
+  Qed.
+
+  Global Instance Eq1_ret_inv_eitherT : Eq1_ret_inv (eitherT E M) :=
+    { eq1_ret_ret := fun a => eq1_ret_ret_eitherT }.
+
+End EitherT.
