src/coq/Utils/MonadReturnsLaws.v
@@ -1,0 +1,60 @@
+From Coq Require Import
+     Morphisms.
+
+From ITree Require Import
+     Basics.Monad.
+
+From ExtLib Require Import
+     Structures.Monads.
+
+From Vellvm.Utils Require Import MonadExcLaws PropT.
+
+Set Primitive Projections.
+
+Section Laws.
+
+  Context (M : Type -> Type).
+  Context {Monad : Monad M}.
+  Context {Eq1 : @Eq1 M}.
+
+  Local Open Scope monad_scope.
+
+  Class MonadReturns :=
+    { MReturns : forall {A} (x : A) (ma : M A), Prop;
+
+      MReturns_bind : forall {A B} (a : A) (b : B) (ma : M A) (k : A -> M B),
+          MReturns a ma -> MReturns b (k a) -> MReturns b (bind ma k);
+
+      MReturns_bind_inv : forall {A B} (ma : M A) (k : A -> M B) (b : B),
+          MReturns b (bind ma k) -> exists a : A , MReturns a ma /\ MReturns b (k a);
+
+      MReturns_ret : forall {A} (a : A) (ma : M A),
+        eq1 ma (ret a) -> MReturns a ma;
+
+      MReturns_ret_inv : forall {A} (x y : A),
+          MReturns x (ret y) -> x = y
+    }.
+
+End Laws.
+
+Arguments MReturns {M _ _ _ _}.
+Arguments MReturns_bind {M _ _ _ _}.
+Arguments MReturns_bind_inv {M _ _ _ _}.
+Arguments MReturns_ret {M _ _ _ _}.
+Arguments MReturns_ret_inv {M _ _ _ _}.
+
+From ITree Require Import
+     ITree
+     Basics.Basics
+     Events.Exception
+     Eq.Eq
+     Events.StateFacts
+     Events.State.
+
+Instance ITree_MonadReturns {E} : MonadReturns (itree E)
+  := { MReturns := fun A => Returns;
+       MReturns_bind := Returns_bind E;
+       MReturns_bind_inv := fun A B => Returns_bind_inversion;
+       MReturns_ret := fun A => ReturnsRet;
+       MReturns_ret_inv := Returns_ret_inv
+     }.
